CrSemantics.v
@@ -1,0 +1,8 @@
+From MyProject Require Export CrIdentifiers.
+From MyProject Require Export CrTransformer.
+
+Class Semantics (T : Type) := {
+  lookup_function_argument : FunctionArgument -> ProgramState T -> T;
+  eval_hdr_op_expr : HdrOp -> ProgramState T -> T;
+  eval_hdr_op_assign : HdrOp -> ProgramState T -> ProgramState T;
+}.
